LambdaS5/coq/LibRel.v
@@ -1,0 +1,138 @@
+(* Heterogenous binary relations *)
+
+Set Implicit Arguments.
+Require Import Utils.
+Require Import LibTactics LibLogic LibBool LibLogic LibProd LibSum LibBagExt.
+Require Export LibOperation.
+Generalizable Variables A B R.
+
+Definition rel A B := A -> B -> Prop.
+
+(* ---------------------------------------------------------------------- *)
+(** ** Inhabited *)
+
+Instance rel_inhab : forall A B, Inhab (rel A B).
+Proof. intros. apply (prove_Inhab (fun _ _ => True)). Qed.
+
+(* ---------------------------------------------------------------------- *)
+(** ** Extensionality *)
+
+Lemma rel_extensional : forall A B (R1 R2:rel A B),
+  (forall x y, R1 x y <-> R2 x y) -> R1 = R2.
+Proof. intros_all. apply~ prop_ext_2. Qed.
+
+Instance rel_extensional_inst : forall A B, Extensional (rel A B).
+Proof. intros. apply (Build_Extensional _ (@rel_extensional A B)). Defined.
+
+(* ---------------------------------------------------------------------- *)
+(** ** Properties *)
+
+Definition sequence {A B C} (R1 : rel A B) (R2 : rel B C) : rel A C := fun x y =>
+    exists z, R1 x z /\ R2 z y.
+
+Section Constructions2.
+Variable (A B : Type).
+Implicit Types R : rel A B.
+Implicit Types a : A.
+Implicit Types b : B.
+
+Definition empty : rel A B := 
+  fun a b => False.
+
+Definition single : A -> B -> rel A B :=
+  fun a b a' b' => a = a' /\ b = b'.
+
+Definition flip R : rel B A :=
+  fun b a => R a b.
+
+Definition compl R : rel A B :=
+  fun a b => ~R a b.
+
+Definition union R1 R2 : rel A B :=
+  fun a b => R1 a b \/ R2 a b. 
+
+Definition inter R1 R2 : rel A B :=
+  fun a b => R1 a b /\ R2 a b. 
+
+Definition incl R1 R2 :=
+  forall a b, R1 a b -> R2 a b.
+
+Definition defined R := 
+  forall a, exists b, R a b.
+
+Definition functional R :=
+  forall a b b', R a b -> R a b' -> b = b'.
+
+End Constructions2.
+
+(* ---------------------------------------------------------------------- *)
+(** ** More on binary relations (to TLC? ) *)  
+
+Section Binary.
+Variable (A : Type).
+Implicit Types R : rel A A.
+Implicit Types x y z : A.
+
+Definition id : rel A A := fun x y => x = y.
+
+Fixpoint pow k (R : rel A A) : rel A A :=
+  match k with
+  | 0 => id
+  | S k' => sequence R (pow k' R)
+  end.
+
+End Binary.
+
+(* ---------------------------------------------------------------------- *)
+(** ** Adapter to LibBag *)
+
+Global Instance union_inst : BagUnion (rel A B) :=
+  { union := @union _ _ }.
+
+Global Instance inter_inst : BagInter (rel A B) :=
+  { inter := @inter _ _ }.
+
+Global Instance empty_inst : BagEmpty (rel A B) :=
+  { empty := @empty _ _ }.
+
+Global Instance single_inst : BagSingle (A * B) (rel A B) :=
+  { single := uncurry2 (@single _ _) }.
+
+Global Instance in_inst : BagIn (A * B) (rel A B) :=
+  { is_in := fun p r => uncurry2 r p }.
+
+Global Instance incl_inst : BagIncl (rel A B) :=
+  { incl := @incl _ _ }.
+
+Global Instance in_empty_eq_inst : In_empty_eq (T := rel A B).
+Proof. constructor. introv. cbv. cases_let. auto. Qed.
+
+Global Instance in_single_eq_inst : In_single_eq (T := rel A B).
+Proof. 
+    constructor. introv. cbv. repeat cases_let.
+    rew_logic. splits; introv Heq.
+    destruct_hyp Heq. reflexivity.
+    injects Heq. auto.
+Qed.
+
+Global Instance in_union_eq_inst : In_union_eq (T := rel A B).
+Proof. constructor. introv. cbv. cases_let. auto. Qed.
+
+Global Instance in_inter_eq_inst : In_inter_eq (T := rel A B).
+Proof. constructor. introv. cbv. cases_let. auto. Qed.
+
+Global Instance in_double_inst : In_double (T := rel A B).
+Proof. 
+    constructor. introv Hr.
+    apply rel_extensional.
+    intros a b. applys Hr (a, b).
+Qed.
+
+Global Instance incl_in_eq_inst : Incl_in_eq (T := rel A B).
+Proof. 
+    constructor. introv. cbv. rew_logic. split; introv Hi.
+    introv. cases_let. auto.
+    intros a b. applys Hi (a, b).
+Qed.    
+
+Global Opaque union_inst inter_inst empty_inst in_inst single_inst incl_inst.
