LambdaS5/coq/LjsShared.v
@@ -1,5 +1,5 @@
 Set Implicit Arguments.
-Require Export LibTactics LibCore LibString LibSet LibFinset LibFinmap.
+Require Export LibTactics LibCore LibString LibSet LibBagExt LibRel LibFinset LibFinmap.
 Generalizable Variables A B.
 Require Export LibProd LibListZ.
 
